src/tidy/rewrite_search/default.lean
@@ -1,0 +1,8 @@
+-- Never import tidy.rewrite_search.engine directly. Go through me.
+import .engine
+
+-- 'tactic.lean' provides the default strategy and tracer (and the tactics)
+import .tactic
+
+import .tracer
+import .strategy
