src/tidy/rewrite_search/tracer/default.lean
@@ -1,0 +1,4 @@
+import .unit
+import .graph
+
+meta def visualiser := tidy.rewrite_search.tracer.graph_tracer
